Widgets demo

widget/dist/htmlDisplay.js
@@ -1,0 +1,66 @@
+import { Fragment as _Fragment, jsx as _jsx, jsxs as _jsxs } from "react/jsx-runtime";
+/*
+Copyright (c) 2022 E.W.Ayers. All rights reserved.
+Released under Apache 2.0 license as described in the file LICENSE.
+Authors: E.W.Ayers, Wojciech Nawrocki
+*/
+import * as React from 'react';
+import { EnvPosContext, importWidgetModule, mapRpcError, useAsyncPersistent, useRpcSession } from '@leanprover/infoview';
+/**
+ * Render a HTML tree into JSX, resolving any dynamic imports corresponding to `component`s along
+ * the way.
+ *
+ * This guarantees that the resulting React tree is exactly as written down in Lean. In particular,
+ * there are no extraneous {@link DynamicComponent} nodes which works better with some libraries
+ * that directly inspect the children nodes.
+ */
+export async function renderHtml(rs, pos, html) {
+    if ('text' in html) {
+        return _jsx(_Fragment, { children: html.text });
+    }
+    else if ('element' in html) {
+        const [tag, attrsList, cs] = html.element;
+        const attrs = {};
+        for (const [k, v] of attrsList) {
+            attrs[k] = v;
+        }
+        const children = await Promise.all(cs.map(async (html) => await renderHtml(rs, pos, html)));
+        if (tag === "hr") {
+            // React is greatly concerned by <hr/>s having children.
+            return _jsx("hr", {});
+        }
+        else if (children.length === 0) {
+            return React.createElement(tag, attrs);
+        }
+        else {
+            return React.createElement(tag, attrs, children);
+        }
+    }
+    else if ('component' in html) {
+        const [hash, export_, props, cs] = html.component;
+        const children = await Promise.all(cs.map(async (html) => await renderHtml(rs, pos, html)));
+        const dynProps = { ...props, pos };
+        const mod = await importWidgetModule(rs, pos, hash);
+        if (!(export_ in mod))
+            throw new Error(`Module '${hash}' does not export '${export_}'`);
+        if (children.length === 0) {
+            return React.createElement(mod[export_], dynProps);
+        }
+        else {
+            return React.createElement(mod[export_], dynProps, children);
+        }
+    }
+    else {
+        return _jsxs("span", { className: "red", children: ["Unknown HTML variant: ", JSON.stringify(html)] });
+    }
+}
+export default function HtmlDisplay({ html }) {
+    const rs = useRpcSession();
+    const pos = React.useContext(EnvPosContext);
+    const state = useAsyncPersistent(() => renderHtml(rs, pos, html), [rs, pos, html]);
+    if (state.state === 'resolved')
+        return state.value;
+    else if (state.state === 'rejected')
+        return _jsxs("span", { className: "red", children: ["Error rendering HTML: ", mapRpcError(state.error).message] });
+    return _jsx(_Fragment, {});
+}
