widget/dist/termDisplayWidget.d.ts
@@ -1,0 +1,6 @@
+interface TermDisplayWidgetProps {
+    term: String;
+    type: String;
+}
+export default function TermDisplayWidget(props: TermDisplayWidgetProps): import("react/jsx-runtime").JSX.Element;
+export {};
