widget/dist/termDisplayWidgetRemote.d.ts
@@ -1,0 +1,27 @@
+import { DocumentPosition, RpcSessionAtPos } from '@leanprover/infoview';
+import type { Name, RpcPtr } from '@leanprover/infoview';
+export type Html = {
+    element: [string, [string, any][], Html[]];
+} | {
+    text: string;
+} | {
+    component: [string, string, any, Html[]];
+};
+/**
+ * Render a HTML tree into JSX, resolving any dynamic imports corresponding to `component`s along
+ * the way.
+ *
+ * This guarantees that the resulting React tree is exactly as written down in Lean. In particular,
+ * there are no extraneous {@link DynamicComponent} nodes which works better with some libraries
+ * that directly inspect the children nodes.
+ */
+export declare function renderHtml(rs: RpcSessionAtPos, pos: DocumentPosition, html: Html): Promise<JSX.Element>;
+export declare function HtmlDisplay({ html }: {
+    html: Html;
+}): JSX.Element;
+interface TermDisplayWidgetRemoteProps {
+    name: Name;
+    env: RpcPtr<'Lean.Environment'>;
+}
+export default function TermDisplayWidgetRemote(props: TermDisplayWidgetRemoteProps): import("react/jsx-runtime").JSX.Element;
+export {};
